Uppaal_Networks/UPPAAL_Asm_AbsInt_Option.thy
@@ -1,0 +1,47 @@
+theory UPPAAL_Asm_AbsInt_Option
+imports UPPAAL_Asm_AbsInt
+begin
+
+instantiation option :: (order) order begin
+  fun less_eq_option :: "('a::order) option \<Rightarrow> 'a option \<Rightarrow> bool" where
+    "less_eq_option None _ \<longleftrightarrow> True" |
+    "less_eq_option (Some x) None \<longleftrightarrow> False" |
+    "less_eq_option (Some x) (Some y) \<longleftrightarrow> x \<le> y"
+  
+  fun less_option :: "'a option \<Rightarrow> 'a option \<Rightarrow> bool" where
+    "less_option None None \<longleftrightarrow> False" |
+    "less_option None (Some x) \<longleftrightarrow> True" |
+    "less_option (Some x) None \<longleftrightarrow> False" |
+    "less_option (Some x) (Some y) \<longleftrightarrow> x < y"
+instance proof
+  show "((x::'a option) < y) = (x \<le> y \<and> \<not> y \<le> x)" for x y by (cases x; cases y) auto
+  show "(x::'a option) \<le> x" for x by (cases x) auto
+  show "(x::'a option) \<le> z" if "x \<le> y" and "y \<le> z" for x y z
+    using that by (cases x; cases y; cases z) auto
+  show "(x::'a option) = y" if "x \<le> y" and "y \<le> x"for x y
+    using that by (cases x; cases y) auto
+qed
+end
+
+instantiation option :: (semilattice_sup) semilattice_sup
+begin
+fun sup_option :: "'a option \<Rightarrow> 'a option \<Rightarrow> 'a option" where
+  "sup_option None b = b" |
+  "sup_option a None = a" |
+  "sup_option (Some a) (Some b) = Some (a \<squnion> b)"
+instance proof
+  show "(x::'a option) \<le> x \<squnion> y" for x y by (cases x; cases y) auto
+  show "(y::'a option) \<le> x \<squnion> y" for x y by (cases x; cases y) auto
+  show "(y::'a option) \<squnion> z \<le> x" if "(y::'a option) \<le> x" "(z::'a option) \<le> x" for x y z using that by (cases x; cases y; cases z) auto
+qed
+end
+
+instantiation option :: (absstate_base) absstate begin
+definition "\<top> \<equiv> Some \<top>"
+instance proof qed end
+
+fun \<gamma>_option :: "('a \<Rightarrow> 'b set) \<Rightarrow> 'a option \<Rightarrow> 'b set" where
+"\<gamma>_option \<gamma> None = {}" |
+"\<gamma>_option \<gamma> (Some a) = \<gamma> a"
+
+end
