Uppaal_Networks/UPPAAL_Asm_AbsInt_State_Dumb.thy
@@ -1,0 +1,44 @@
+theory UPPAAL_Asm_AbsInt_State_Dumb
+imports UPPAAL_Asm_AbsInt UPPAAL_Asm_AbsInt_Option
+begin
+
+datatype dumb_base = Any
+
+lemma dumb_base_is_dumb: "(x::dumb_base) = y" for x y by (cases x; cases y) blast
+
+instantiation dumb_base :: absstate_base
+begin
+  definition "\<top> \<equiv> Any"
+  fun less_eq_dumb_base :: "dumb_base \<Rightarrow> dumb_base \<Rightarrow> bool" where "less_eq_dumb_base _ _ \<longleftrightarrow> True"
+  fun less_dumb_base :: "dumb_base \<Rightarrow> dumb_base \<Rightarrow> bool" where "less_dumb_base _ _ \<longleftrightarrow> False"
+  fun sup_dumb_base :: "dumb_base \<Rightarrow> dumb_base \<Rightarrow> dumb_base" where "sup_dumb_base _ _  = Any"
+instance by standard (auto simp: dumb_base_is_dumb)
+end
+
+type_synonym dumb = "dumb_base option"
+
+fun \<gamma>_dumb :: "dumb \<Rightarrow> collect_state set" where
+  "\<gamma>_dumb v  = \<gamma>_option (\<lambda>_. \<top>) v"
+
+global_interpretation AbsState
+where \<gamma> = \<gamma>_dumb
+proof (standard, goal_cases)
+  case (1 a b)
+  then show ?case
+  proof (cases a)
+    case (Some aa)
+    then show ?thesis
+    proof (cases b)
+      case None
+      then show ?thesis using 1 using Some less_eq_option.simps(2) by blast
+    next
+      case (Some bb)
+      then show ?thesis by (cases bb) auto
+    qed
+  qed simp
+next
+  case 2
+  then show ?case by (simp add: top_dumb_base_def top_option_def)
+qed
+
+end
